Syntax.v
@@ -1,39 +1,53 @@
-Require Export unscoped.
+Require Import Base.
 
-From Coq Require Vectors.Vector.
-Module V := Vector.
-Notation vec := (fun n A => V.t A n).
-
-Class signature := {
+Structure signature := {
     FuncS : Type;
-    fun_arr : FuncS -> nat;
+    fun_ar : FuncS -> nat;
     PredS : Type;
-    pred_arr : PredS -> nat;
+    pred_ar : PredS -> nat;
     IndPredS : Type;
-    indpred_arr : IndPredS -> nat;
-    }.
+    indpred_ar : IndPredS -> nat
+  }.
 
-Arguments FuncS {Σ} : rename.
-Arguments PredS {Σ} : rename.
-Arguments IndPredS {Σ} : rename.
+Arguments fun_ar {Σ} f : rename.
+Arguments pred_ar {Σ} P : rename.
+Arguments indpred_ar {Σ} P : rename.
 
+Notation var := fin.
 Section term.
   Context {Σ : signature}.
 
+  Unset Elimination Schemes.
+  
   Inductive term  : Type :=
   | var_term : fin -> term 
-  | TFunc : forall (f : FuncS), ( vec (fun_arr f) (term  ) ) -> term .
+  | TFunc : forall (f : FuncS Σ), vec term (fun_ar f) -> term .
+  
+  Set Elimination Schemes.
 
-  Lemma congr_TFunc { f : FuncS }  { s0 : vec (fun_arr f) (term  ) } { t0 : vec (fun_arr f) (term  ) } (H1 : s0 = t0) : TFunc  f s0 = TFunc  f t0 .
+  Inductive TV : term -> E.Ensemble var :=
+  | TVVar : forall v, TV (var_term v) v
+  | TVFunc : forall f args v, (exists st, V.In st args /\ TV st v) ->
+                          TV (TFunc f args) v.
+  
+  Lemma congr_TFunc
+    {f : FuncS Σ}
+    {s0 : vec term (fun_ar f)}
+    {t0 : vec term (fun_ar f)}
+    (H1 : s0 = t0)
+    : TFunc  f s0 = TFunc  f t0 .
   Proof. congruence. Qed.
 
-  Fixpoint subst_term   (sigmaterm : fin -> term ) (s : term ) : term  :=
-    match s return term  with
-    | var_term  s => sigmaterm s
-    | TFunc  f s0 => TFunc  f ((V.map (subst_term sigmaterm)) s0)
+  Fixpoint subst_term  (sigmaterm : fin -> term) (s : term) : term :=
+    match s return term with
+    | var_term s => sigmaterm s
+    | TFunc f s0 => TFunc f (V.map (subst_term sigmaterm) s0)
     end.
 
-  Definition up_term_term   (sigma : fin -> term ) : fin -> term  :=
+  Definition term_var_subst (t : term) (x : var) (u : term) : term :=
+    subst_term (fun v => if v =? x then u else var_term v) t.
+  
+  Definition up_term_term  (sigma : fin -> term) : fin -> term  :=
     (scons) ((var_term ) (var_zero)) ((funcomp) (subst_term ((funcomp) (var_term ) (shift))) sigma).
 
   Definition upId_term_term  (sigma : fin -> term ) (Eq : forall x, sigma x = (var_term ) x) : forall x, (up_term_term sigma) x = (var_term ) x :=
@@ -41,14 +55,6 @@ Section term.
           | S fin_n => (ap) (subst_term ((funcomp) (var_term ) (shift))) (Eq fin_n)
           | 0  => eq_refl
           end.
-
-  (* Added manually. *)
-  Definition vec_id {A : Type} {f : A -> A} (Hid : forall x, f x = x) :
-    forall {n} (v : vec n A), V.map f v = v.
-    intros n v. induction v.
-    - reflexivity.
-    - simpl. rewrite IHv. rewrite Hid. reflexivity.
-  Defined.
   
   Fixpoint idSubst_term  (sigmaterm : fin -> term ) (Eqterm : forall x, sigmaterm x = (var_term ) x) (s : term ) : subst_term sigmaterm s = s :=
     match s return subst_term sigmaterm s = s with
@@ -62,14 +68,6 @@ Section term.
              | 0  => eq_refl
              end.
 
-  Definition vec_ext {A B} {f g : A -> B} :
-    (forall x, f x = g x) -> forall {n} (v : vec n A),  V.map f v = V.map g v.
-    intros Heq n; induction v.
-    - reflexivity.
-    - cbn. f_equal.
-      + apply Heq.
-      + apply IHv.
-  Defined.
   
   Fixpoint ext_term   (sigmaterm : fin -> term ) (tauterm : fin -> term ) (Eqterm : forall x, sigmaterm x = tauterm x) (s : term ) : subst_term sigmaterm s = subst_term tauterm s :=
     match s return subst_term sigmaterm s = subst_term tauterm s with
@@ -77,15 +75,6 @@ Section term.
     | TFunc  f s0 => congr_TFunc ((vec_ext (ext_term sigmaterm tauterm Eqterm)) s0)
     end.
 
-  Definition vec_comp {A B C} {f: A -> B} {g: B -> C} {h} :
-    (forall x, (funcomp g f) x = h x) ->
-    forall {n} (v : vec n A), V.map g (V.map f v) = V.map h v.
-  Proof.
-    intros Heq n; induction v.
-    - reflexivity.
-    - cbn. rewrite <- Heq. f_equal. apply IHv.
-  Defined.
-  
   Fixpoint compSubstSubst_term    (sigmaterm : fin -> term ) (tauterm : fin -> term ) (thetaterm : fin -> term ) (Eqterm : forall x, ((funcomp) (subst_term tauterm) sigmaterm) x = thetaterm x) (s : term ) : subst_term tauterm (subst_term sigmaterm s) = subst_term thetaterm s :=
     match s return subst_term tauterm (subst_term sigmaterm s) = subst_term thetaterm s with
     | var_term  s => Eqterm s
@@ -98,10 +87,10 @@ Section term.
              | 0  => eq_refl
              end.
 
-  Lemma instId_term  : subst_term (var_term ) = id .
+  Lemma instId_term  : subst_term var_term = id .
   Proof. exact ((FunctionalExtensionality.functional_extensionality _ _ ) (fun x => idSubst_term (var_term ) (fun n => eq_refl) ((id) x))). Qed.
 
-  Lemma varL_term   (sigmaterm : fin -> term ) : (funcomp) (subst_term sigmaterm) (var_term ) = sigmaterm .
+  Lemma varL_term   (sigmaterm : fin -> term) : (funcomp) (subst_term sigmaterm) (var_term ) = sigmaterm .
   Proof. exact ((FunctionalExtensionality.functional_extensionality _ _ ) (fun x => eq_refl)). Qed.
 
   Lemma compComp_term    (sigmaterm : fin -> term ) (tauterm : fin -> term ) (s : term ) : subst_term tauterm (subst_term sigmaterm s) = subst_term ((funcomp) (subst_term tauterm) sigmaterm) s .
@@ -112,20 +101,99 @@ Section term.
 
 End term.
 
+Arguments term Σ : clear implicits.
+
+Section term_ind.
+  Context {Σ : signature} (P : term Σ -> Prop).
+  
+  Hypothesis Pbase : forall v, P (var_term v).
+  Hypothesis Pind : forall (f : FuncS Σ) args,
+      (forall st, V.In st args -> P st) -> P (TFunc f args).
+
+  Definition term_ind : forall t, P t.
+    fix IND_PRINCIPLE 1; intros [v | f args].
+    - apply Pbase.
+    - apply Pind. apply V.Forall_forall.         
+      induction args; constructor.
+      + apply IND_PRINCIPLE.
+      + assumption.
+  Defined.
+End term_ind.
+
+Section term_facts.
+  Context {Σ : signature}.
+
+  Lemma var_not_in_TV_not_eq : forall v x, ~ @TV Σ (var_term v) x -> v <> x.
+  Proof.
+    intros v x H. intros eq. apply H. subst; constructor.
+  Qed.
+  
+  Lemma var_not_in_Func_not_in_args : forall (f : FuncS Σ) args x,
+      ~ TV (TFunc f args) x -> forall st, V.In st args -> ~ TV st x.
+  Proof.
+    intros f args x Hnotin; unfold E.In in *.
+    intros t Hin Hvar. apply Hnotin.
+    apply TVFunc.
+    exists t; intuition.
+  Qed.
+    
+  Lemma term_subst_id : forall (t : term Σ) (x : var),
+      subst_term (fun x => var_term x) t = t.
+  Proof.
+    pose proof (@idSubst_term Σ) as idsubst.
+    intros t v. apply idsubst. intuition.
+  Qed.
+    
+  Lemma term_var_subst_no_occ : forall (t u : term Σ) (x : var),
+      ~ TV t x -> term_var_subst t x u = t.
+  Proof.
+    intros t; induction t as [v | f args IH];
+      intros u x Hnotin; cbn.
+    - destruct (v =? x) eqn:E.
+      + exfalso; apply Hnotin; rewrite Nat.eqb_eq in E; subst; constructor.
+      + reflexivity.
+    - f_equal. rewrite <- V.map_id. apply V.map_ext_in.
+      intros st Hstin. apply IH.
+      + assumption.
+      + intros Hinvar. apply Hnotin. constructor.
+        exists st; intuition.
+  Qed.                                             
+End term_facts.
+
 Section formula.
   Context {Σ : signature}.
   
   Inductive formula  : Type :=
-  | FPred : forall (P : PredS), ( vec (pred_arr P) (term  ) ) -> formula 
-  | FIndPred : forall (P : IndPredS), ( vec (indpred_arr P) (term  ) ) -> formula 
-  | FNeg : ( formula   ) -> formula 
-  | FImp : ( formula   ) -> ( formula   ) -> formula 
-  | FAll : ( formula   ) -> formula .
+  | FPred : forall (P : PredS Σ), vec (term Σ) (pred_ar P) -> formula 
+  | FIndPred : forall (P : IndPredS Σ), vec (term Σ) (indpred_ar P) -> formula 
+  | FNeg : formula -> formula 
+  | FImp : formula -> formula -> formula 
+  | FAll : formula -> formula .
 
-  Lemma congr_FPred { P : PredS }  { s0 : vec (pred_arr P) (term  ) } { t0 : vec (pred_arr P) (term  ) } (H1 : s0 = t0) : FPred  P s0 = FPred  P t0 .
+  Inductive FV : formula -> E.Ensemble var :=
+  | FV_Pred : forall R args v, (forall st, V.In st args -> ~ TV st v) ->
+                          FV (FPred R args) v
+  | FV_IndPred : forall R args v, (forall st, V.In st args -> ~ TV st v) ->
+                             FV (FIndPred R args) v
+  | FV_Imp_l : forall F G v, FV F v -> FV (FImp F G) v
+  | FV_Imp_r : forall F G v, FV G v -> FV (FImp F G) v
+  | FV_Neg : forall F v, FV F v -> FV (FNeg F) v
+  | FV_All : forall F v, FV F v -> FV (FAll F) (S v).
+  
+  Lemma congr_FPred
+    {P : PredS Σ}
+    {s0 : vec (term Σ) (pred_ar P)}
+    {t0 : vec (term Σ) (pred_ar P)}
+    (H1 : s0 = t0)
+    : FPred  P s0 = FPred  P t0 .
   Proof. congruence. Qed.
 
-  Lemma congr_FIndPred { P : IndPredS }  { s0 : vec (indpred_arr P) (term  ) } { t0 : vec (indpred_arr P) (term  ) } (H1 : s0 = t0) : FIndPred  P s0 = FIndPred  P t0 .
+  Lemma congr_FIndPred
+    {P : IndPredS Σ}
+    {s0 : vec (term Σ) (indpred_ar P)}
+    {t0 : vec (term Σ) (indpred_ar P)}
+    (H1 : s0 = t0)
+    : FIndPred  P s0 = FIndPred  P t0 .
   Proof. congruence. Qed.
 
   Lemma congr_FNeg  { s0 : formula   } { t0 : formula   } (H1 : s0 = t0) : FNeg  s0 = FNeg  t0 .
@@ -137,7 +205,7 @@ Section formula.
   Lemma congr_FAll  { s0 : formula   } { t0 : formula   } (H1 : s0 = t0) : FAll  s0 = FAll  t0 .
   Proof. congruence. Qed.
 
-  Fixpoint subst_formula   (sigmaterm : fin -> term ) (s : formula ) : formula  :=
+  Fixpoint subst_formula   (sigmaterm : fin -> term Σ) (s : formula ) : formula  :=
     match s return formula  with
     | FPred  P s0 => FPred  P ((V.map (subst_term sigmaterm)) s0)
     | FIndPred  P s0 => FIndPred  P ((V.map (subst_term sigmaterm)) s0)
@@ -146,7 +214,7 @@ Section formula.
     | FAll  s0 => FAll  ((subst_formula (up_term_term sigmaterm)) s0)
     end.
 
-  Fixpoint idSubst_formula  (sigmaterm : fin -> term ) (Eqterm : forall x, sigmaterm x = (var_term ) x) (s : formula ) : subst_formula sigmaterm s = s :=
+  Fixpoint idSubst_formula  (sigmaterm : fin -> term Σ) (Eqterm : forall x, sigmaterm x = (var_term ) x) (s : formula ) : subst_formula sigmaterm s = s :=
     match s return subst_formula sigmaterm s = s with
     | FPred  P s0 => congr_FPred ((vec_id (idSubst_term sigmaterm Eqterm)) s0)
     | FIndPred  P s0 => congr_FIndPred ((vec_id (idSubst_term sigmaterm Eqterm)) s0)
@@ -155,7 +223,7 @@ Section formula.
     | FAll  s0 => congr_FAll ((idSubst_formula (up_term_term sigmaterm) (upId_term_term (_) Eqterm)) s0)
     end.
 
-  Fixpoint ext_formula   (sigmaterm : fin -> term ) (tauterm : fin -> term ) (Eqterm : forall x, sigmaterm x = tauterm x) (s : formula ) : subst_formula sigmaterm s = subst_formula tauterm s :=
+  Fixpoint ext_formula   (sigmaterm : fin -> term Σ) (tauterm : fin -> term Σ) (Eqterm : forall x, sigmaterm x = tauterm x) (s : formula ) : subst_formula sigmaterm s = subst_formula tauterm s :=
     match s return subst_formula sigmaterm s = subst_formula tauterm s with
     | FPred  P s0 => congr_FPred ((vec_ext (ext_term sigmaterm tauterm Eqterm)) s0)
     | FIndPred  P s0 => congr_FIndPred ((vec_ext (ext_term sigmaterm tauterm Eqterm)) s0)
@@ -164,7 +232,7 @@ Section formula.
     | FAll  s0 => congr_FAll ((ext_formula (up_term_term sigmaterm) (up_term_term tauterm) (upExt_term_term (_) (_) Eqterm)) s0)
     end.
 
-  Fixpoint compSubstSubst_formula    (sigmaterm : fin -> term ) (tauterm : fin -> term ) (thetaterm : fin -> term ) (Eqterm : forall x, ((funcomp) (subst_term tauterm) sigmaterm) x = thetaterm x) (s : formula ) : subst_formula tauterm (subst_formula sigmaterm s) = subst_formula thetaterm s :=
+  Fixpoint compSubstSubst_formula    (sigmaterm : fin -> term Σ) (tauterm : fin -> term Σ) (thetaterm : fin -> term Σ) (Eqterm : forall x, ((funcomp) (subst_term tauterm) sigmaterm) x = thetaterm x) (s : formula ) : subst_formula tauterm (subst_formula sigmaterm s) = subst_formula thetaterm s :=
     match s return subst_formula tauterm (subst_formula sigmaterm s) = subst_formula thetaterm s with
     | FPred  P s0 => congr_FPred ((vec_comp (compSubstSubst_term sigmaterm tauterm thetaterm Eqterm)) s0)
     | FIndPred  P s0 => congr_FIndPred ((vec_comp (compSubstSubst_term sigmaterm tauterm thetaterm Eqterm)) s0)
@@ -176,33 +244,20 @@ Section formula.
   Lemma instId_formula  : subst_formula (var_term ) = id .
   Proof. exact ((FunctionalExtensionality.functional_extensionality _ _ ) (fun x => idSubst_formula (var_term ) (fun n => eq_refl) ((id) x))). Qed.
 
-  Lemma compComp_formula    (sigmaterm : fin -> term ) (tauterm : fin -> term ) (s : formula ) : subst_formula tauterm (subst_formula sigmaterm s) = subst_formula ((funcomp) (subst_term tauterm) sigmaterm) s .
+  Lemma compComp_formula    (sigmaterm : fin -> term Σ) (tauterm : fin -> term Σ) (s : formula ) : subst_formula tauterm (subst_formula sigmaterm s) = subst_formula ((funcomp) (subst_term tauterm) sigmaterm) s .
   Proof. exact (compSubstSubst_formula sigmaterm tauterm (_) (fun n => eq_refl) s). Qed.
 
-  Lemma compComp'_formula    (sigmaterm : fin -> term ) (tauterm : fin -> term ) : (funcomp) (subst_formula tauterm) (subst_formula sigmaterm) = subst_formula ((funcomp) (subst_term tauterm) sigmaterm) .
+  Lemma compComp'_formula    (sigmaterm : fin -> term Σ) (tauterm : fin -> term Σ ) : (funcomp) (subst_formula tauterm) (subst_formula sigmaterm) = subst_formula ((funcomp) (subst_term tauterm) sigmaterm) .
   Proof. exact ((FunctionalExtensionality.functional_extensionality _ _ ) (fun n => compComp_formula sigmaterm tauterm n)). Qed.
 
 End formula.
 
 
+Instance Subst_term (Σ : signature)  : Subst1 (fin -> term Σ) (term Σ) (term Σ) := @subst_term Σ   .
 
+Instance Subst_formula (Σ : signature)  : Subst1 (fin -> term Σ) (formula ) (formula ) := @subst_formula Σ  .
 
-
-
-
-
-
-
-
-
-
-
-
-Global Instance Subst_term (Σ : signature)  : Subst1 (fin -> term ) (term ) (term ) := @subst_term Σ   .
-
-Global Instance Subst_formula (Σ : signature)  : Subst1 (fin -> term ) (formula ) (formula ) := @subst_formula Σ  .
-
-Global Instance VarInstance_term (Σ : signature) : Var (fin) (term ) := @var_term Σ .
+Instance VarInstance_term (Σ : signature) : Var (fin) (term Σ) := @var_term Σ .
 
 Notation "x '__term'" := (var_term x) (at level 5, format "x __term") : subst_scope.
 
@@ -216,7 +271,7 @@ Notation "↑__term" := (up_term) (only printing) : subst_scope.
 
 Notation "↑__term" := (up_term_term) (only printing) : subst_scope.
 
-Global Instance Up_term_term (Σ : signature)  : Up_term (_) (_) := @up_term_term Σ  .
+Instance Up_term_term (Σ : signature)  : Up_term (_) (_) := @up_term_term Σ  .
 
 Notation "s [ sigmaterm ]" := (subst_term sigmaterm s) (at level 7, left associativity, only printing) : subst_scope.
 
