Base.v
@@ -1,5 +1,6 @@
 Require Export Utf8.
 Require Export Arith Bool.
+Require Export unscoped.
 
 Require Vectors.Vector.
 Module V := Vector.
@@ -12,8 +13,8 @@ Require Sets.Ensembles.
 Module E := Ensembles.
 Arguments E.In {U} A x.
 
-Lemma Exists_exists : forall A (P : A -> Prop) n (v : V.t A n),
-    V.Exists P v <-> (exists a : A, V.In a v /\ P a).
+Lemma vec_Exists_exists : forall A (P : A -> Prop) n (v : vec A n),
+    V.Exists P v <-> ex (fun t => V.In t v /\ P t).
 Proof.
   intros A P n v; split.
   - intros Hex; induction Hex.
@@ -23,3 +24,28 @@ Proof.
     + apply V.Exists_cons_hd; assumption.
     + apply V.Exists_cons_tl; assumption.
 Qed.
+
+Definition vec_id {A : Type} {f : A -> A} (Hid : forall x, f x = x) :
+  forall {n} (v : vec A n), V.map f v = v.
+  intros n v. induction v.
+  - reflexivity.
+  - simpl. rewrite IHv. rewrite Hid. reflexivity.
+Defined.
+
+Definition vec_ext {A B} {f g : A -> B} :
+  (forall x, f x = g x) -> forall {n} (v : vec A n),  V.map f v = V.map g v.
+  intros Heq n; induction v.
+  - reflexivity.
+  - cbn. f_equal.
+    + apply Heq.
+    + apply IHv.
+Defined.
+
+Definition vec_comp {A B C} {f: A -> B} {g: B -> C} {h} :
+  (forall x, (funcomp g f) x = h x) ->
+  forall {n} (v : vec A n), V.map g (V.map f v) = V.map h v.
+Proof.
+  intros Heq n; induction v.
+  - reflexivity.
+  - cbn. rewrite <- Heq. f_equal. apply IHv.
+Defined.
